@prefix owl: <http://www.w3.org/2002/07/owl#> .
@prefix rdf: <http://www.w3.org/1999/02/22-rdf-syntax-ns#> .
@prefix xml: <http://www.w3.org/XML/1998/namespace> .
@prefix xsd: <http://www.w3.org/2001/XMLSchema#> .
@prefix odrl: <http://www.w3.org/ns/odrl/2/> .
@prefix rdfs: <http://www.w3.org/2000/01/rdf-schema#> .
@prefix profile: <http://www.w3.org/ns/dx/prof/> .
@prefix skos: <http://www.w3.org/2004/02/skos/core#> .
@prefix vann: <http://purl.org/vocab/vann/> .
@prefix dcterms: <http://purl.org/dc/terms/> .

@prefix tosl: <http://isagroup/tosl/> .


<http://isagroup/tosl> a owl:Ontology, profile:Profile ;
            profile:isProfileOf <http://www.w3.org/ns/odrl/2/core> ;
            rdfs:comment "This is the RDF ontology for the ODLR profile Terms of Service language" ;
            rdfs:label "ODLR Terms of Service Language Profile Version 1" ;
            dcterms:abstract "Abstract." ;
            dcterms:contributor "ISA-Group" ;
            dcterms:created "2024-11-27"^^xsd:date ;
            dcterms:creator "Elena Molino Peña", "José María Cruz", "José María García", "Antonio Ruiz Cortés" ;
            dcterms:description "The ODLR Profile for Terms of Service Language (TOSL) enhances the understanding and enforcement of legal terms within service agreements. Utilizing the Open Digital Rights Language (ODLR), this profile specifies the obligations, rights, and prohibitions contained in agreements to effectively identify and flag potentially unfair terms. By integrating ODLR's flexible framework, the TSL profile aims to ensure clearer, more enforceable, and fairer terms of service agreements across diverse digital platforms." ;
            dcterms:license <https://dalicc.net/licenselibrary/CC-BY-4.0> ;
            dcterms:title "Terms of Service Language Ontology" ;
            dcterms:modified "2024-01-17"^^xsd:date ;
            vann:preferredNamespacePrefix "tosl" ;
            vann:preferredNamespaceUri "http://www.w3.org/tosl/"^^xsd:string ;
            owl:versionInfo "1"^^xsd:string .

#################################################################
#    Object Properties
#################################################################

###  http://isagroup/tosl/onDispute
tosl:onDispute a rdf:type, owl:ObjectProperty, skos:Concept ;
            rdfs:domain odrl:Policy ;
            rdfs:range tosl:DisputeResolution ; 
            rdfs:isDefinedBy <http://isagroup/tosl/> ;
            rdfs:label "Arbitration" ;
            skos:definition "Represents the relationship between a Policy and its associated Dispute Resolution mechanism, specifying how, where, and under which law disputes arising under the Policy will be resolved" .
            

###  http://isagroup/tosl/condition
tosl:condition a rdf:type, owl:ObjectProperty, skos:Concept ;
           rdfs:domain tosl:DisputeResolution ;
           rdfs:range [ rdf:type owl:Class ;
                        owl:unionOf ( odrl:Constraint
                                      odrl:LogicalConstraint
                                    )
                      ] ;
           rdfs:isDefinedBy <http://isagroup/tosl/> ;
           rdfs:label "Has Condition" ;
           skos:definition "This relationship enables the specification of particular restrictions that apply to the dispute" .


###  http://isagroup/tosl/governedBy
tosl:governedBy a rdf:type, owl:ObjectProperty, skos:Concept ;
            rdfs:domain tosl:DisputeResolution ;
            rdfs:range tosl:Law ;
            rdfs:isDefinedBy <http://isagroup/tosl/> ;
            rdfs:label "Governed By" ;
            skos:definition "Establishes the connection to the specific legal framework that governs the agreement" .


###  http://isagroup/tosl/liability
tosl:liability a rdf:type, owl:ObjectProperty, skos:Concept ;
           rdfs:domain odrl:Policy , odrl:Asset,
                       odrl:Rule ;
           rdfs:range tosl:Liability ;
           rdfs:isDefinedBy <http://isagroup/tosl/> ;
           rdfs:label "With Liability" ;
           skos:definition "Establishes the relationship between a rule, policy or asset and the applicable liabilities, describing the duties or obligations to be assumed in a specific context" .


###  http://isagroup/tosl/liableParty
tosl:liableParty a rdf:type, owl:ObjectProperty, skos:Concept ;
             rdfs:domain tosl:Liability ;
             rdfs:range odrl:Party ;
             rdfs:isDefinedBy <http://isagroup/tosl/> ;
             rdfs:label "Liable Party" ;
             skos:definition "This term establishes the connection between liability and a party to whom they apply" .


###  http://isagroup/tosl/limitation
tosl:limitation a rdf:type, owl:ObjectProperty, skos:Concept ;
            rdfs:domain tosl:Liability ;
            rdfs:range [ rdf:type owl:Class ;
                         owl:unionOf ( odrl:Constraint
                                       odrl:LogicalConstraint
                                     )
                       ] ;
            rdfs:isDefinedBy <http://isagroup/tosl/> ;
            rdfs:label "Has Limitation" ;
            skos:definition "Defines a relationship that allows specifying particular restrictions or conditions related to the limitation of liabilities of a party" .


###  http://isagroup/tosl/limitationOfLiability
tosl:limitationOfLiability a rdf:type, owl:ObjectProperty, skos:Concept ;
                       rdfs:domain odrl:Policy , odrl:Asset,
                                   odrl:Rule ;
                       rdfs:range tosl:Liability ;
                       rdfs:isDefinedBy <http://isagroup/tosl/> ;
                       rdfs:label "With Limitation Of Liability" ;
                       skos:definition "Defines the relationship that links a rule, policy or asset to the limitations of liability applicable to one or more parties, specifying the scope and restrictions in cases of damages or breaches" .


###  http://isagroup/tosl/requires
tosl:requires a rdf:type, owl:ObjectProperty, skos:Concept ;
          rdfs:domain tosl:Litigation ;
          rdfs:range tosl:Arbitration ;
          rdfs:isDefinedBy <http://isagroup/tosl/> ;
          rdfs:label "Requires" ;
          skos:definition "This relationship specifies that all disputes must be resolved through arbitration" .


###  http://isagroup/tosl/takesPlaceIn
tosl:takesPlaceIn a rdf:type, owl:ObjectProperty, skos:Concept ;
              rdfs:domain tosl:DisputeResolution ;
              rdfs:range tosl:Jurisdiction ;
              rdfs:isDefinedBy <http://isagroup/tosl/> ;
              rdfs:label "Takes Place In" ;
              skos:definition "This term describes the relationship between Dispute Resolution and Jurisdiction, specifying the location where disputes are to be resolved" .


###  http://isagroup/tosl/triggers
tosl:triggers a rdf:type, owl:ObjectProperty, skos:Concept ;
          rdfs:domain odrl:Permission ;
          rdfs:range odrl:Duty ;
          rdfs:isDefinedBy <http://isagroup/tosl/> ;
          rdfs:label "Triggers" ;
          skos:definition "Represents the relationship where a permission can trigger a specific duty for a party" .


#################################################################
#    Classes
#################################################################

###  http://isagroup/tosl/Arbitration
tosl:Arbitration a rdf:type, owl:Class, skos:Concept ;
             rdfs:subClassOf tosl:DisputeResolution ;
             rdfs:isDefinedBy <http://isagroup/tosl/> ;
             rdfs:label "Arbitration" ;
             skos:definition "Arbitration is a process for resolving disputes without recourse to conventional judicial systems, typically managed by an arbitrator" .


###  http://isagroup/tosl/DisputeResolution
tosl:DisputeResolution a rdf:type, owl:Class, skos:Concept ;
                   rdfs:isDefinedBy <http://isagroup/tosl/> ;
                   rdfs:label "Dispute Resolution" ;
                   skos:definition "Employed to specify the mechanisms for resolving disputes among the parties involved in the agreement" .


###  http://isagroup/tosl/Jurisdiction
tosl:Jurisdiction a rdf:type, owl:Class, skos:Concept ;
              rdfs:isDefinedBy <http://isagroup/tosl/> ;
              rdfs:label "Jurisdiction" ;
              skos:definition "Jurisdiction refers to the specific location or legal authority where a dispute must be resolved" .


###  http://isagroup/tosl/Law
tosl:Law a rdf:type, owl:Class, skos:Concept ;
     rdfs:isDefinedBy <http://isagroup/tosl/> ;
     rdfs:label "Law" ;
     skos:definition "Law refers to the specific statutes and regulations that govern an agreement and are applicable in resolving any disputes arising from it" .


###  http://isagroup/tosl/Liability
tosl:Liability a rdf:type, owl:Class, skos:Concept ;
           rdfs:isDefinedBy <http://isagroup/tosl/> ;
           rdfs:label "Liability" ;
           skos:definition "Liability refers to the specific provisions that define and restrict the extent to which each party in the agreement can be held accountable for damages or losses" ;
           skos:note """ Example of use: 
           tosl:liability [
        a tosl:Liability ;
        rdf:value tosl:physicalInjuries ;
        tosl:party :elsevier ;
    ] ;
    tosl:limitationOfLiability [
        a tosl:Liability ;
        rdf:value tosl:anyDamage ;
        tosl:party :customer ;
        tosl:limitation [
            a odrl:Constraint ;
            odrl:leftOperand tosl:maximunCompensation ;
            odrl:operator odrl:lt ;
            odrl:rightOperand 1000 ;
            dcterm:unit \\\"USD\\\" ;
        ]
    ] ;""" .


###  http://isagroup/tosl/Litigation
tosl:Litigation a rdf:type, owl:Class, skos:Concept ;
            rdfs:subClassOf tosl:DisputeResolution ;
            rdfs:isDefinedBy <http://isagroup/tosl/> ;
            rdfs:label "Litigation" ;
            skos:definition "Litigation is a legal process in which the provider or customer, acting as the plaintiff, initiates proceedings against the other party, called the defendant, before a civil court in a settlement dispute" .

###  http://isagroup/tosl/Service
tosl:Service a rdf:type, owl:Class, skos:Concept ;
         rdfs:subClassOf odrl:Asset ;
         rdfs:isDefinedBy <http://isagroup/tosl/> ;
         rdfs:label "Service"@en ;
         skos:definition "An asset that includes the service affected by the action as a resource"@en .


###  http://isagroup/tosl/UserContent
tosl:UserContent a rdf:type, owl:Class, skos:Concept ;
             rdfs:subClassOf odrl:Asset ;
             rdfs:isDefinedBy <http://isagroup/tosl/> ;
             rdfs:label "User Content"@en ;
             skos:definition "An asset that encompasses either all or part of a user's content"@en .


#################################################################
#    Individuals
#################################################################

###  http://isagroup/tosl/remove
tosl:remove a rdf:type, owl:NamedIndividual, skos:Concept,
                 odrl:Action ;
        rdfs:isDefinedBy <http://isagroup/tosl/> ;
        rdfs:label "Remove" ;
        skos:definition "This action may authorize, obligate, or prohibit the deletion of content from the provided services" .


###  http://isagroup/tosl/consent
tosl:consent a rdf:type, owl:NamedIndividual, skos:Concept,
                  odrl:Action ;
         rdfs:isDefinedBy <http://isagroup/tosl/> ;
         rdfs:label "Consent" ;
         skos:definition "This action signifies your acceptance of the associated asset" .


###  http://isagroup/tosl/allowDownload
tosl:allowDownload a rdf:type, owl:NamedIndividual, skos:Concept,
                        odrl:Action ;
               rdfs:isDefinedBy <http://isagroup/tosl/> ;
               rdfs:label "Allow Download" ;
               skos:definition "Allow download refers to the action that permits one of the parties, typically the client, to download personal information or information about contracted services" .


###  http://isagroup/tosl/terminate
tosl:terminate a rdf:type, owl:NamedIndividual, skos:Concept,
                    odrl:Action ;
           rdfs:isDefinedBy <http://isagroup/tosl/> ;
           rdfs:label "Terminate" ;
           skos:definition "This action permits the termination of an asset, whether it be the agreement, services, or any other associated entity" .
           

###  http://isagroup/tosl/publish
tosl:publish a rdf:type, owl:NamedIndividual, skos:Concept,
                 odrl:Action ;
         rdfs:isDefinedBy <http://isagroup/tosl/> ;
         rdfs:label "Publish" ;
         skos:definition "This action mandates the public release of an asset" .


###  http://isagroup/tosl/integrate
tosl:integrate a rdf:type, owl:NamedIndividual, skos:Concept,
                                          odrl:Action ;
                                 odrl:includedIn odrl:use ;
                                 rdfs:isDefinedBy <http://isagroup/tosl/> ;
                                 rdfs:label "Integrate" ;
                                 skos:definition "This action allows, obligates, or prohibits the integration of the provided service with your application." .


###  http://isagroup/tosl/develop
tosl:develop a rdf:type, owl:NamedIndividual, skos:Concept,
                                        odrl:Action ;
                               odrl:includedIn odrl:use ;
                               dcterms:description "This action permits, mandates or prohibits the use of the services to develop a software application." ;
                               rdfs:isDefinedBy <http://isagroup/tosl/> ;
                               rdfs:label "Develop" .


###  http://isagroup/tosl/test
tosl:test a rdf:type, owl:NamedIndividual, skos:Concept,
                                     odrl:Action ;
                            odrl:includedIn odrl:use ;
                            dcterms:description "This action permits, mandates or prohibits the use of the services to test a software application." ;
                            rdfs:isDefinedBy <http://isagroup/tosl/> ;
                            rdfs:label "Test" .


###  http://isagroup/tosl/anyLiability
tosl:anyLiability a rdf:type, owl:NamedIndividual, skos:Concept,
                    tosl:Liability ;
           rdfs:isDefinedBy <http://isagroup/tosl/> ;
           rdfs:label "Any Damage" ;
           skos:definition "This liability provision specifies that the designated party may or may not be held liable for damages caused by the other party." .


###  http://isagroup/tosl/physicalInjuries
tosl:physicalInjuries a rdf:type, owl:NamedIndividual, skos:Concept,
                           tosl:Liability ;
                  rdfs:isDefinedBy <http://isagroup/tosl/> ;
                  rdfs:label "Physical Injuries" ;
                  skos:definition "This provision outlines the liability of the party in cases of physical damages caused to the other party" .


###  http://isagroup/tosl/harmCausedByMalware
tosl:harmCausedByMalware a rdf:type, owl:NamedIndividual, skos:Concept,
                              tosl:Liability ;
                     rdfs:isDefinedBy <http://isagroup/tosl/> ;
                     rdfs:label "Harm Caused By Malware" ;
                     skos:definition "The party is or not is responsible for any damages resulting from malware" .

    
###  http://isagroup/tosl/justification
tosl:justification a rdf:type, owl:NamedIndividual, skos:Concept,
                              odrl:LeftOperand ;
             rdfs:isDefinedBy <http://isagroup/tosl/> ;
             rdfs:label "Justification" ;
             skos:definition "This condition mandates that specific actions can only be undertaken with appropriate justification" .


###  http://isagroup/tosl/priorNotice
tosl:priorNotice a rdf:type, owl:NamedIndividual, skos:Concept,
                              odrl:LeftOperand ;
                     rdfs:isDefinedBy <http://isagroup/tosl/> ;
                     rdfs:label "Prior Notice" ;
                     skos:definition "This stipulates that the parties must give advance notice before certain actions are taken" .


###  http://isagroup/tosl/consentType
tosl:consentType a rdf:type, owl:NamedIndividual, skos:Concept,
                      odrl:LeftOperand ;
             rdfs:isDefinedBy <http://isagroup/tosl/> ;
             rdfs:label "Consent Type" ;
             skos:definition "This term refers to the specific manner in which consent is given by a party within an agreement, outlining whether it is implicit, explicit, or expressed through other defined actions" .


###  http://isagroup/tosl/compliesWith
tosl:compliesWith a rdf:type, owl:NamedIndividual, skos:Concept,
                       odrl:LeftOperand ;
              rdfs:isDefinedBy <http://isagroup/tosl/> ;
              rdfs:label "Complies With" ;
              skos:definition  "The use of the services requires adherence to specific conditions and obligations outlined by the service provider" .


###  http://isagroup/tosl/causes
tosl:causes a rdf:type, owl:NamedIndividual, skos:Concept,
                       odrl:LeftOperand ;
              rdfs:isDefinedBy <http://isagroup/tosl/> ;
              rdfs:label "Causes" ;
              skos:definition "Indicates that the specified action produces a direct effect or consequence on the target of the Rule. This operand is used to establish a cause-effect relationship where the action leads to a measurable impact on an asset" ;
              skos:note """This LeftOperand is intended to be paired with RightOperands that define the type or extent of the impact, such as degradation, alteration, or enhancement. For example, "causes eq degradation" signifies that the action leads to a significant degradation in a specified metric of the target, such as performance, security, or availability""" .


###  http://isagroup/tosl/implicitConsent
tosl:implicitConsent a rdf:type, owl:NamedIndividual, skos:Concept,
                         odrl:RightOperand ;
                rdfs:isDefinedBy <http://isagroup/tosl/> ;
                rdfs:label "Implicit Consent" ;
                skos:definition "This type of consent implies that by merely utilizing the service, the customer agrees to the terms of the agreement by default" .


###  http://isagroup/tosl/explicitConsent
tosl:explicitConsent a rdf:type, owl:NamedIndividual, skos:Concept,
                           odrl:RightOperand ;
                  rdfs:isDefinedBy <http://isagroup/tosl/> ;
                  rdfs:label "Explicit Consent" ;
                  skos:definition "This form of consent requires that the customer explicitly affirm or accept the agreement through a formal action, such as signing a document" .


###  http://isagroup/tosl/degradation
tosl:degradation a rdf:type, owl:NamedIndividual, skos:Concept,
                           odrl:RightOperand ;
                  rdfs:isDefinedBy <http://isagroup/tosl/> ;
                  rdfs:label "Degradation" ;
                  skos:definition "Indicates a significant and unreasonable degradation of some metric, such as response time or availability, caused by the action of the Rule to the target of the Rule" ;
                  skos:note """This RightOperand is intended to be used in conjunction with LeftOperands that specify actions or events impacting performance metrics. An example is "causes eq degradation", which expresses that the exertion of the action MUST not cause a service significant degradation""" .


###  http://isagroup/tosl/consumerPlaceLaw
tosl:consumerPlaceLaw a rdf:type, owl:NamedIndividual, skos:Concept,
                           tosl:Law ;
                  rdfs:isDefinedBy <http://isagroup/tosl/> ;
                  rdfs:label "Consumer Place Law" ;
                  skos:definition "This provision states that the law governing the agreement is that of the consumer's country or the law that affects the consumer" .


###  http://isagroup/tosl/californiaLaw
tosl:californiaLaw a rdf:type, owl:NamedIndividual, skos:Concept,
                        tosl:Law ;
               rdfs:isDefinedBy <http://isagroup/tosl/> ;
               rdfs:label "California Law" ;
               skos:definition "This instance denotes that the governing law applicable to the agreement is that of California" .


###  http://isagroup/tosl/europeanLaw
tosl:europeanLaw a rdf:type, owl:NamedIndividual, skos:Concept,
                      tosl:Law ;
             rdfs:isDefinedBy <http://isagroup/tosl/> ;
             rdfs:label "European Law" ;
             skos:definition "this stipulates that the law regulating the agreement is European law" .
